spinlock based on tokens

pulse/lib/pulse/lib/Pulse.Lib.SpinLockToken.fst
@@ -43,12 +43,7 @@ fn new_lock (v:vprop { is_big v })
   let t1 = T.witness (L.iref_of l);
   let i = new_invariant (exists* (p:perm). L.lock_active #p l);
   let t2 = T.witness i;
-  let l = {
-    l;
-    i;
-    t1;
-    t2
-  };
+  let l = { l; i; t1; t2 };
   l
 }
 ```
@@ -57,9 +52,9 @@ let lock_acquired (#v:vprop) (l:lock v) : vprop =
   L.lock_acquired l.l
 
 ```pulse
-fn acquire (#v:vprop) (l:lock v)
+fn lock_alive (#v:vprop) (l:lock v)
   requires emp
-  ensures v ** lock_acquired l
+  ensures exists* (p:perm). L.lock_alive l.l #p v
 {
   T.recall l.t2;
   with_invariants l.i
@@ -73,9 +68,32 @@ fn acquire (#v:vprop) (l:lock v)
   with p. assert (L.lock_active #p l.l);
   L.elim_inv_and_active_into_alive l.l v #p;
   elim_stick _ _;
-  drop_ (inv _ _);
+  drop_ (inv _ _)
+}
+```
+
+```pulse
+fn acquire (#v:vprop) (l:lock v)
+  requires emp
+  ensures v ** lock_acquired l
+{
+  lock_alive l;
+  with p. assert (L.lock_alive l.l #p v);
   L.acquire l.l;
   fold (lock_acquired l);
+  drop_ (L.lock_alive l.l #p v)
+}
+```
+
+```pulse
+fn release (#v:vprop) (l:lock v)
+  requires v ** lock_acquired l
+  ensures emp
+{
+  lock_alive l;
+  with p. assert (L.lock_alive l.l #p v);
+  unfold (lock_acquired l);
+  L.release l.l;
   drop_ (L.lock_alive l.l #p v)
 }
 ```
